Refactor/generalize some pipeline definitions/proofs
When we do rewriting after casts, we will need to do extra passes of DCE
and subst01 to fully reduce things, so we generalize some of the interp
proofs over cast behavior.

For ease of rewriting, we make [ident.interp] an alias (notation) for
[ident.gen_interp], rather than a [Definition].

We also factor out the rewriting wrapper inside the pipeline module into
its own definition.

src/Experiments/NewPipeline/Language.v
@@ -1021,13 +1021,11 @@ Module Compilers.
 
       Definition cast_outside_of_range (r : zrange) (v : BinInt.Z) : BinInt.Z.
       Proof. exact v. Qed.
-
-      (** Interpret identifiers where [Z_cast] is an opaque identity
-         function when the value is not inside the range *)
-      Definition interp {t} (idc : ident t) : type.interp base.interp t
-        := @gen_interp cast_outside_of_range t idc.
-      Global Arguments interp _ !_ / .
     End with_base.
+
+    (** Interpret identifiers where [Z_cast] is an opaque identity
+        function when the value is not inside the range *)
+    Notation interp := (@gen_interp cast_outside_of_range).
     Notation LiteralUnit := (@Literal base.type.unit).
     Notation LiteralZ := (@Literal base.type.Z).
     Notation LiteralBool := (@Literal base.type.bool).
@@ -1297,14 +1295,13 @@ Module Compilers.
       Notation "x || y" := (#Z_lor @ x @ y)%expr : expr_scope.
       Notation "x 'mod' y" := (#Z_modulo @ x @ y)%expr : expr_scope.
       Notation "- x" := (#Z_opp @ x)%expr : expr_scope.
-      Global Arguments interp _ !_.
       Global Arguments gen_interp _ _ !_.
     End Notations.
   End ident.
   Export ident.Notations.
   Notation ident := ident.ident.
 
-  Global Strategy -1000 [expr.Interp expr.interp ident.interp type.interp base.interp base.base_interp ident.gen_interp].
+  Global Strategy -1000 [expr.Interp expr.interp type.interp base.interp base.base_interp ident.gen_interp].
   Ltac reify var term :=
     expr.reify base.type ident ltac:(base.reify) ident.reify var term.
   Ltac Reify term :=
